Foundation/InterpretabilityLogic/Veltman/AxiomJ1.lean
@@ -1,0 +1,38 @@
+import Foundation.InterpretabilityLogic.Veltman.Basic
+
+namespace LO.InterpretabilityLogic.Veltman
+
+open Veltman Formula.Veltman
+
+variable {F : Veltman.Frame} {φ ψ χ : Formula ℕ}
+
+namespace Frame
+
+class HasAxiomJ1 (F : Frame) : Prop where
+  S_refl : ∀ x, IsRefl _ (F.S x)
+export HasAxiomJ1 (S_refl)
+
+end Frame
+
+@[simp high, grind]
+lemma validate_axiomJ1_of_J1 [F.HasAxiomJ1] : F ⊧ Axioms.J1 φ ψ := by
+  intro V x h y hy;
+  use y;
+  constructor;
+  . apply F.S_refl x |>.refl;
+  . apply h;
+    . exact y.2;
+    . exact hy;
+
+lemma Frame.HasAxiomJ1.of_validate_axiomJ1 (h : F ⊧ Axioms.J1 (.atom 0) (.atom 1)) : F.HasAxiomJ1 := by
+  constructor;
+  intro x;
+  constructor;
+  intro y;
+  obtain ⟨z, Sxyz, hz⟩ := @h (λ u _ => u = y) x (by tauto) y (by tauto);
+  replace hz : z = y := by
+    simp only [Satisfies] at hz;
+    grind;
+  apply hz ▸ Sxyz;
+
+end LO.InterpretabilityLogic.Veltman
