Foundation/InterpretabilityLogic/Veltman/Hilbert.lean
@@ -1,4 +1,5 @@
 import Foundation.InterpretabilityLogic.Hilbert.Basic.Basic
+import Foundation.InterpretabilityLogic.Hilbert.Minimal.Basic
 import Foundation.InterpretabilityLogic.Veltman.Basic
 
 namespace LO.InterpretabilityLogic
@@ -6,12 +7,43 @@ namespace LO.InterpretabilityLogic
 open Formula
 open Formula.Veltman
 
-namespace Veltman
-
 variable {Ax Ax₁ Ax₂ : Axiom ℕ} {φ : Formula ℕ}
-variable {F : Frame} {C : FrameClass}
+variable {F : Veltman.Frame} {C C₁ C₂ : Veltman.FrameClass}
 
-lemma soundness_of_validates_axioms (hGL : ∀ F ∈ C, F.IsGL) (hV : C ⊧* Ax) : Hilbert.Basic Ax ⊢ φ → C ⊧ φ := by
+namespace Hilbert.Minimal.Veltman
+
+lemma soundness_frameclass (hV : C ⊧* Ax) : Hilbert.Minimal Ax ⊢ φ → C ⊧ φ := by
+  intro hφ F hF;
+  induction hφ using Hilbert.Minimal.rec! with
+  | @axm φ s h =>
+    apply ValidOnFrame.subst;
+    apply hV.models;
+    . assumption;
+    . assumption;
+  | _ => grind;
+
+instance instFrameClassSound (hV : C ⊧* Ax) : Sound (Hilbert.Minimal Ax) C := ⟨fun {_} => soundness_frameclass hV⟩
+
+lemma consistent_of_sound_frameclass
+  (C : Veltman.FrameClass) (C_nonempty: C.Nonempty)
+  [sound : Sound (Hilbert.Minimal Ax) C]
+  : Entailment.Consistent (Hilbert.Minimal Ax) := by
+  apply Entailment.Consistent.of_unprovable (φ := ⊥);
+  apply not_imp_not.mpr sound.sound;
+  apply Semantics.set_models_iff.not.mpr;
+  push_neg;
+  obtain ⟨F, hF⟩ := C_nonempty;
+  use F;
+  constructor;
+  . assumption;
+  . simp;
+
+end Hilbert.Minimal.Veltman
+
+
+namespace Hilbert.Basic.Veltman
+
+lemma soundness_frameclass (hV : C ⊧* Ax) : Hilbert.Basic Ax ⊢ φ → C ⊧ φ := by
   intro hφ F hF;
   induction hφ using Hilbert.Basic.rec! with
   | @axm φ s h =>
@@ -19,17 +51,9 @@ lemma soundness_of_validates_axioms (hGL : ∀ F ∈ C, F.IsGL) (hV : C ⊧* Ax)
     apply hV.models;
     . assumption;
     . assumption;
-  | mdp ihpq ihp => exact ValidOnFrame.mdp ihpq ihp;
-  | nec ih => exact ValidOnFrame.nec ih;
-  | imply₁ => exact ValidOnFrame.imply₁;
-  | imply₂ => exact ValidOnFrame.imply₂;
-  | ec => exact ValidOnFrame.elimContra;
-  | axiomK => exact ValidOnFrame.axiomK;
-  | axiomL => have := hGL F hF; exact ValidOnFrame.axiomL;
+  | _ => grind;
 
-instance instSound_of_validates_axioms (hGL : ∀ F ∈ C, F.IsGL) (hV : C ⊧* Ax) : Sound (Hilbert.Basic Ax) C := ⟨fun {_} =>
-  soundness_of_validates_axioms hGL hV
-⟩
+instance instFrameClassSound (hV : C ⊧* Ax) : Sound (Hilbert.Basic Ax) C := ⟨fun {_} => soundness_frameclass hV⟩
 
 lemma consistent_of_sound_frameclass
   (C : Veltman.FrameClass) (C_nonempty: C.Nonempty)
@@ -46,32 +70,26 @@ lemma consistent_of_sound_frameclass
   . simp;
 
 
-lemma soundness_of_frame_validates_axioms [F.IsGL] (hV : F ⊧* Ax) : (Hilbert.Basic Ax) ⊢ φ → F ⊧ φ := by
+lemma soundness_frame [F.IsGL] (hV : F ⊧* Ax) : (Hilbert.Basic Ax) ⊢ φ → F ⊧ φ := by
   intro hφ;
   induction hφ using Hilbert.Basic.rec! with
   | axm s h =>
     apply ValidOnFrame.subst;
     apply hV.models;
     assumption;
-  | mdp ihpq ihp => exact ValidOnFrame.mdp ihpq ihp;
-  | nec ih => exact ValidOnFrame.nec ih;
-  | imply₁ => exact ValidOnFrame.imply₁;
-  | imply₂ => exact ValidOnFrame.imply₂;
-  | ec => exact ValidOnFrame.elimContra;
-  | axiomK => exact ValidOnFrame.axiomK;
-  | axiomL => exact ValidOnFrame.axiomL;
+  | _ => grind;
 
-instance instSound_of_frame_validates_axioms [F.IsGL] (hV : F ⊧* Ax) : Sound (Hilbert.Basic Ax) F := ⟨fun {_} =>
-  soundness_of_frame_validates_axioms hV
+instance instFrameSound [F.IsGL] (hV : F ⊧* Ax) : Sound (Hilbert.Basic Ax) F := ⟨fun {_} =>
+  soundness_frame hV
 ⟩
 
-lemma consistent_of_sound_frames (F : Veltman.Frame) [sound : Sound (Hilbert.Basic Ax) F] : Entailment.Consistent (Hilbert.Basic Ax) := by
+lemma consistent_of_sound_frame (F : Veltman.Frame) [sound : Sound (Hilbert.Basic Ax) F] : Entailment.Consistent (Hilbert.Basic Ax) := by
   apply Entailment.Consistent.of_unprovable (φ := ⊥);
   apply not_imp_not.mpr sound.sound;
   exact Veltman.ValidOnFrame.bot_def;
 
 lemma weakerThan_of_subset_frameClass
-  (C₁ C₂ : FrameClass) (hC : C₂ ⊆ C₁)
+  (C₁ C₂ : Veltman.FrameClass) (hC : C₂ ⊆ C₁)
   [Sound (Hilbert.Basic Ax₁) C₁] [Complete (Hilbert.Basic Ax₂) C₂]
   : (Hilbert.Basic Ax₁) ⪯ (Hilbert.Basic Ax₂) := by
   apply Entailment.weakerThan_iff.mpr;
@@ -81,20 +99,7 @@ lemma weakerThan_of_subset_frameClass
   apply Sound.sound (𝓜 := C₁) hφ;
   apply hC hF;
 
-/-
-lemma validates_CL_axioms_union (hV : C ⊧* Ax) : C ⊧* CL.axioms ∪ Ax := by
-  constructor;
-  rintro φ ((rfl | rfl | rfl | rfl | rfl | rfl) | hφ);
-  . intro _ _; apply ValidOnFrame.axiomK;
-  . intro _ _; apply ValidOnFrame.axiomL;
-  . intro _ _; apply ValidOnFrame.axiomJ1;
-  . intro _ _; apply ValidOnFrame.axiomJ2;
-  . intro _ _; apply ValidOnFrame.axiomJ3;
-  . intro _ _; apply ValidOnFrame.axiomJ4;
-  . apply hV.models;
-    assumption;
--/
+end Hilbert.Basic.Veltman
 
-end Veltman
 
 end LO.InterpretabilityLogic
