Foundation/InterpretabilityLogic/Veltman/Logic/ILMinus.lean
@@ -1,0 +1,38 @@
+import Foundation.InterpretabilityLogic.Veltman.Hilbert
+
+namespace LO.InterpretabilityLogic
+
+open Veltman
+
+
+namespace Veltman
+
+protected abbrev FrameClass.ILMinus : FrameClass := Set.univ
+
+abbrev trivialFrame : Veltman.Frame where
+  toKripkeFrame := Modal.Kripke.blackpoint
+  S _ _ _ := True
+
+end Veltman
+
+
+namespace ILMinus
+
+open Hilbert.Minimal.Veltman
+
+instance Veltman.sound : Sound InterpretabilityLogic.ILMinus FrameClass.ILMinus := by
+  apply instFrameClassSound;
+  constructor;
+  intro φ hφ F hF;
+  replace hF := Set.mem_setOf_eq.mp hF;
+  rcases hφ with (rfl | rfl | rfl | rfl) <;> simp;
+
+instance : Entailment.Consistent InterpretabilityLogic.ILMinus := consistent_of_sound_frameclass FrameClass.ILMinus $ by
+  use Veltman.trivialFrame;
+  apply Set.mem_setOf_eq.mpr;
+  simp;
+
+end ILMinus
+
+
+end LO.InterpretabilityLogic
