Foundation/InterpretabilityLogic/Veltman/Logic/ILMinus_J1.lean
@@ -1,0 +1,37 @@
+import Foundation.InterpretabilityLogic.Veltman.Logic.ILMinus
+import Foundation.InterpretabilityLogic.Veltman.AxiomJ1
+
+namespace LO.InterpretabilityLogic
+
+open Veltman
+
+
+namespace Veltman
+
+protected abbrev FrameClass.ILMinus_J1 : FrameClass := { F | F.HasAxiomJ1 }
+
+instance : trivialFrame.HasAxiomJ1 where
+  S_refl _ := ⟨by tauto⟩
+
+end Veltman
+
+
+namespace ILMinus_J1
+
+open Hilbert.Minimal
+
+instance Veltman.sound : Sound InterpretabilityLogic.ILMinus_J1 FrameClass.ILMinus_J1 := by
+  apply Veltman.instFrameClassSound;
+  constructor;
+  intro φ hφ F hF;
+  replace hF := Set.mem_setOf_eq.mp hF;
+  rcases (by simpa [buildAxioms] using hφ) with (rfl | rfl | rfl | rfl) <;> simp;
+
+instance : Entailment.Consistent InterpretabilityLogic.ILMinus_J1 := Veltman.consistent_of_sound_frameclass FrameClass.ILMinus_J1 $ by
+  use Veltman.trivialFrame;
+  apply Set.mem_setOf_eq.mpr;
+  infer_instance;
+
+end ILMinus_J1
+
+end LO.InterpretabilityLogic
